theories/KatInc.v
@@ -1,0 +1,529 @@
+(** * imp: a formalisation of the IMP programming language on top of KAT *)
+
+(* We formalise the IMP language (whose programs are also known as
+   "while programs"). We give a big step semantics as an inductive
+   predicate, and using KAT, and we show that the two versions
+   actually coincide.
+   
+   We then use the [kat] tactic to prove some simple program
+   equivalences, and to derive all rules of corresponding Hoare logic
+   for partial correctness. *)
+
+From Stdlib Require Import ZArith.
+From RelationAlgebra Require Import kat prop rel comparisons kat_tac relalg.
+
+Section s.
+(** identifiers for memory locations  *)
+Variable loc: Set.
+(** abstract state (or memory) *)
+Variable state: Set.
+(** updating the state *)
+Variable update: loc -> Z -> state -> state.
+
+(** * Definition of the languague *)
+
+(** programs *)
+
+Inductive prog :=
+| skp
+| aff (x: loc) (e: state -> Z)
+| seq (p q: prog)
+| ite (t: dset state) (p q: prog)
+| whl (t: dset state) (p: prog).
+
+(** notations *)
+Declare Scope imp_scope.
+Bind Scope imp_scope with prog.
+Delimit Scope imp_scope with imp.
+Notation "x  <- y" := (aff x y) (at level 90): imp_scope.
+Notation "p  ;; q" := (seq p%imp q%imp) (left associativity, at level 101): imp_scope.
+Arguments ite _%_ra _%_imp _%_imp.
+Arguments whl _%_ra _%_imp.
+
+
+(** * Big step semantics *)
+
+(** corresponding functional relation *)
+Notation upd x e := (frel (fun s => update x (e s) s)).
+
+
+(** ** using KAT expressions in the model of relations
+
+   the semantics can then be given by induction on the program, using
+   a simple fixpoint *)
+
+Fixpoint bstep (p: prog): hrel state state :=
+  match p with
+    | skp => 1
+    | aff x e => upd x e
+    | seq p q => bstep p ⋅ bstep q
+    | ite b p q => [b] ⋅ bstep p + [!b] ⋅ bstep q
+    | whl b p => ([b] ⋅ bstep p)^*  ⋅  [!b]
+  end.
+
+(** ** using an inductive predicate, as in standard textbooks *)
+
+Inductive bstep': prog -> hrel state state :=
+| s_skp: forall s, bstep' skp s s
+| s_aff: forall x e s, bstep' (x <- e) s (update x (e s) s)
+| s_seq: forall p q s s' s'', bstep' p s s' -> bstep' q s' s'' -> bstep' (p ;; q) s s''
+| s_ite_ff: forall (b: dset state) p q s s', b s = false -> bstep' q s s' -> bstep' (ite b p q) s s'
+| s_ite_tt: forall (b: dset state) p q s s', b s = true -> bstep' p s s' -> bstep' (ite b p q) s s'
+| s_whl_ff: forall (b: dset state) p s, b s = false -> bstep' (whl b p) s s
+| s_whl_tt: forall (b: dset state) p s s', b s = true -> bstep' (p ;; whl b p) s s' -> bstep' (whl b p) s s'.
+
+(** ** equivalence between the two definitions *)
+
+Lemma bstep_eq p: bstep' p ≡ bstep p.
+Proof.
+  apply antisym. 
+  - intros s s'. induction 1. 
+     reflexivity. 
+     reflexivity. 
+     eexists; eassumption. 
+     right. eexists. split. reflexivity. simpl; now rewrite H. assumption.
+     left. eexists. split. reflexivity. assumption. assumption. 
+     exists s. apply (str_refl ([b] ⋅ bstep p)). reflexivity.
+      simpl. unfold hrel_inj. simpl. now rewrite H.
+     destruct IHbstep' as [t ? [t' ? ?]]. exists t'. 2: assumption. 
+     apply (str_cons ([b] ⋅ bstep p)). exists t. 2: assumption.
+     eexists; eauto. now split. 
+  - induction p; unfold bstep; fold bstep.
+     intros ? ? <-. constructor. 
+     intros ? ? ->. constructor. 
+     intros ? ? [? H1 H2]. econstructor. apply IHp1, H1. apply IHp2, H2.
+     intros ? ? [[? [<- H] H']|[? [<- H] H']]. 
+      apply s_ite_tt. assumption. apply IHp1, H'. 
+      apply s_ite_ff. now apply Bool.negb_true_iff. apply IHp2, H'. 
+     apply str_ind_l'.
+      intros ? ? [<- H]. apply s_whl_ff. now apply Bool.negb_true_iff.
+      rewrite <-dotA. intros s s'' [? [<- H] [s' H' H'']]. apply s_whl_tt. assumption.
+      econstructor. apply IHp, H'. assumption.
+Qed. 
+
+
+(** * Some program equivalences *)
+
+(** two programs are said to be equivalent if they have the same semantics *)
+Notation "p ~ q" := (bstep p ≡ bstep q) (at level 80). 
+
+(** ad-hoc simplification tactic *)
+Ltac simp := unfold bstep; fold bstep.
+
+
+(** ** denesting nested loops *)
+Lemma two_loops b p: 
+  whl b (whl b p)  ~  whl b p.
+Proof. simp. kat. Qed.
+
+(** ** folding a loop *)
+Lemma fold_loop b p: 
+  whl b (p ;; ite b p skp)  ~  
+  whl b p.
+Proof. simp. kat. Qed.
+
+(** ** eliminating deadcode *)
+Lemma dead_code b p q r: 
+  (whl b p ;; ite b q r)  ~  
+  (whl b p ;; r).
+Proof. simp. kat. Qed.
+
+Lemma dead_code' a b p q r: 
+  (whl (a ⊔ b) p ;; ite b q r)  ~ 
+  (whl (a ⊔ b) p ;; r).
+Proof. simp. kat. Qed.
+
+
+(** * Reasoning about assignations *)
+
+(** (higher-order style) substitution in formulas and expressions *)
+Definition subst x v (A: dset state): dset state := 
+  fun s => A (update x (v s) s).
+Definition esubst x v (e: state -> Z): state -> Z :=
+  fun s => e (update x (v s) s).
+
+(** is [x] fresh in the expression e *)
+Definition fresh x (e: state -> Z) := forall v s, e (update x v s) = e s.
+
+Hypothesis update_twice: forall x i j s, update x j (update x i s) = update x j s.
+Hypothesis update_comm: forall x y i j s, x<>y -> update x i (update y j s) = update y j (update x i s).
+
+
+(** ** stacking assignations *)
+
+Lemma aff_stack x e f:
+  (x <- e ;; x <- f)  ~  
+  (x <- esubst x e f).
+Proof.
+  simp. rewrite frel_comp.
+  apply frel_weq; intro s. 
+  apply update_twice.
+Qed.
+
+
+(** ** removing duplicates *)
+
+Lemma aff_idem x e: fresh x e -> (x <- e ;; x <- e)  ~  (x <- e). 
+Proof. 
+  intro. rewrite aff_stack. 
+  intros s s'. cbv. rewrite (H (e s)). tauto.
+Qed.
+
+(** ** commuting assignations *)
+
+Lemma aff_comm x y e f: x<>y  -> fresh y e ->  
+  (x <- e ;; y <- f)  ~ (y <- esubst x e f ;; x <- e).
+Proof.
+  intros Hx Hy. simp. rewrite 2frel_comp. apply frel_weq; intro s.
+  rewrite update_comm by congruence. 
+  now rewrite (Hy _). 
+Qed.
+
+(** ** delaying choices *)
+
+(** in the above example, we cannot exploit KAT since this is just
+   about assignations. In the following example, we show how to
+   perform a mixed proof: once we assert that the test [t] somehow
+   commutes with the assignation [x<-e], [hkat] can make use of this
+   assumption to close the goal *)
+
+Lemma aff_ite x e t p q: 
+  (x <- e ;; ite t p q)  
+  ~ 
+  (ite (subst x e t) (x <- e ;; p) (x <- e ;; q)).
+Proof.
+  simp. 
+  assert (H: upd x e ⋅ [t] ≡ [subst x e t] ⋅ upd x e)
+   by (cbv; firstorder; subst; eauto). 
+  hkat.
+Qed.
+
+
+
+(** * Embedding Hoare logic for partial correctness *)
+
+(** Hoare triples for partial correctness can be expressed really
+   easily using KAT: *)
+Notation Hoare A p B := ([A] ⋅ bstep p ⋅ [!B] ≦ 0).
+
+(** ** correspondence w.r.t. the standard interpretation of Hoare triples  *)
+Lemma Hoare_eq A p B: 
+  Hoare A p B <-> 
+  forall s s', A s -> bstep p s s' -> B s'.
+Proof.
+  split. 
+  - intros H s s' HA Hp. case_eq (B s'). reflexivity. intro HB. 
+    destruct (H s s'). exists s'. exists s. 
+    now split. assumption. split. reflexivity. simpl. now rewrite HB. 
+  - intros H s s' [? [? [<- HA] Hp] [-> HB]]. simpl in HB. 
+    rewrite (H _ _ HA Hp) in HB. discriminate. 
+Qed.
+
+
+
+(** ** deriving Hoare logic rules using the [hkat] tactic *)
+
+(** Hoare triples are encoded as propositions of the shape [x ≦ 0] ;
+   therefore, they can always be eliminated by [hkat], so that all
+   rules of Hoare logic can be proved automatically (except for the
+   assignation rule, of course) 
+
+   This idea come from the following paper:
+   Dexter Kozen. On Hoare logic and Kleene algebra with tests. 
+   Trans. Computational Logic, 1(1):60-76, July 2000.
+   
+   The fact that we have an automatic tactic makes it trivial to
+   formalise it. *)
+
+Lemma weakening (A A' B B': dset state) p: 
+  A' ≦ A -> Hoare A p B -> B ≦ B' -> Hoare A' p B'.
+Proof. hkat. Qed.
+
+Lemma rule_skp A: Hoare A skp A.
+Proof. simp. kat. Qed.
+
+Lemma rule_seq A B C p q: 
+  Hoare A p B -> 
+  Hoare B q C -> 
+  Hoare A (p;;q) C.
+Proof. simp. hkat. Qed.
+
+Lemma rule_ite A B t p q: 
+  Hoare (A ⊓ t) p B -> 
+  Hoare (A ⊓ !t) q B -> 
+  Hoare A (ite t p q) B.
+Proof. simp. hkat. Qed.
+
+Lemma rule_whl A t p: 
+  Hoare (A ⊓ t) p A -> 
+  Hoare A (whl t p) (A ⊓ neg t).
+Proof. simp. hkat. Qed.
+
+Lemma rule_aff x v (A: dset state): Hoare (subst x v A) (x <- v) A.
+Proof. 
+  rewrite Hoare_eq. intros s s' HA H. 
+  now inversion_clear H.
+Qed.
+
+Lemma wrong_rule_whl A t p: 
+  Hoare (A ⊓ !t) p A -> 
+  Hoare A (whl t p) (A ⊓ !t).
+Proof. simp. Fail hkat. Abort.
+
+Lemma rule_whl' (I A: dset state) t p: 
+  Hoare (I ⊓ t) p I -> 
+  I ⊓ !t ≦ A -> 
+  Hoare I (whl t p) A.
+Proof. eauto 3 using weakening, rule_whl. Qed.
+
+
+
+
+(** * Embedding Incorrectness logic for normal termination
+
+   Following Zhang, Azevedo de Amorim and Gaboardi (POPL 2022), the
+   incorrectness triple [B] p [C] of O'Hearn (2020) can be encoded
+   equationally in Kleene algebra with tests extended with a top
+   element ⊤ (Kleene Algebra with Top and Tests, or TopKAT):
+
+       [B] p [C]   ≜   ⊤ ⋅ B ⋅ p  ≥  C
+
+   Intuitively, ⊤ ⋅ x captures the codomain of [x]: in the model of
+   binary relations, [⊤ ⋅ x] is the complete relation on the domain
+   restricted to [cod(x)]. Hence the encoding above states
+   [cod(B; bstep p) ⊇ cod(C)], i.e. every state satisfying [C] is
+   reachable from some state satisfying [B] by running [p].
+
+   The current development does not provide a dedicated TopKAT
+   abstract structure, but the relational model [hrel state state] is
+   already a TopKAT: it inherits a bounded distributive lattice
+   structure (level [BDL]), so it has a top element [top: hrel state state]
+   which is the complete relation [fun s s' => True].
+   The two key facts we use are:
+   - [dottx]: [x ≦ ⊤ ⋅ x]   (since [1 ≦ ⊤])
+   - [top_nnm]: [⊤ ⋅ ⊤ ≡ ⊤]   (idempotence of ⊤ under composition)
+   *)
+
+(** ** Incorrectness triples *)
+
+Notation Incorrectness B p C := ([C] ≦ top ⋅ [B] ⋅ bstep p).
+
+(** ** Correspondence with the standard (relational) interpretation *)
+
+Lemma Incorrectness_eq B p C:
+  Incorrectness B p C <->
+  forall s', C s' -> exists2 s, B s & bstep p s s'.
+Proof.
+  split.
+  - intros H s' HC.
+    destruct (H s' s') as [k Hk Hp].
+    { split. reflexivity. simpl. case_eq (C s'). reflexivity.
+      intro Hcs'. rewrite Hcs' in HC. discriminate HC. }
+    destruct Hk as [j _ Hjk]. simpl in Hjk. destruct Hjk as [Hjk HB].
+    subst k. exists j. exact HB. exact Hp.
+  - intros H s s' [Hss HC]. subst s'.
+    destruct (H s HC) as [s0 HB Hp].
+    exists s0.
+    + exists s0. exact I. split. reflexivity. exact HB.
+    + exact Hp.
+Qed.
+
+(** ** Deriving the rules of incorrectness logic
+
+   Unlike the Hoare-logic rules above, these rules cannot be discharged
+   by the [kat]/[hkat] tactic, since these tactics ignore the top
+   element. They are however straightforward consequences of the
+   underlying TopKAT identities. *)
+
+(** An [hkat]-like tactic for IL rules in TopKAT shape.
+    The "trick" beyond plain [hkat] is to pose [top_nnm] as a hypothesis
+    so [hkat] can use [⊤·⊤ ≡ ⊤] during normalization. *)
+Ltac ikat_chain :=
+  repeat match goal with
+         | H : _ ≦ top ⋅ _ ⋅ bstep _ |- _ => rewrite H
+         end.
+
+(** [ikat]: an [hkat]-style wrapper for IL goals in TopKAT shape.
+    Handles:
+      - empty postcondition (rule_iempty);
+      - disjunctive pre/post (rule_idisj);
+      - any goal closed by [lattice]/[kat]/[hkat] after [simp] or after
+        folding [top·top → top] via [top_nnm].
+    Does *not* handle: rules requiring transitivity-chaining through
+    [Incorrectness] hypotheses (e.g. rule_iseq), or rules essentially
+    proved via the semantic form [Incorrectness_eq] (rule_iskp,
+    rule_iite_*, rule_iwhl_*, rule_iaff). *)
+Ltac ikat :=
+  intros;
+  simp;
+  first
+    [ now (rewrite inj_bot; apply leq_bx)
+    | now lattice
+    | now hkat
+    | now (rewrite top_nnm; hkat)
+    | now kat
+    | (* disjunctive shape: [A1 ⊔ A2] / [C1 ⊔ C2] *)
+      now (rewrite ?inj_cup, ?dotxpls, ?dotplsx;
+           apply leq_cupx; ikat_chain; lattice)
+    | idtac "ikat: cannot close goal" ].
+
+(** *** Empty *)
+Lemma rule_iempty A p: Incorrectness A p bot.
+Proof. ikat. Qed.
+
+(** *** Consequence (note the contravariance: in Incorrectness, the
+   precondition gets weaker, the postcondition gets stronger) *)
+Lemma rule_iconseq (A A' B B': dset state) p:
+  A ≦ A' -> Incorrectness A p B -> B' ≦ B -> Incorrectness A' p B'.
+Proof.
+  intros HA H HB. rewrite HB, H.
+  apply dot_leq. 2: reflexivity.
+  apply dot_leq. reflexivity.
+  apply inj_leq, HA.
+Qed.
+
+(** *** Disjunction *)
+Lemma rule_idisj (A1 A2 C1 C2: dset state) p:
+  Incorrectness A1 p C1 ->
+  Incorrectness A2 p C2 ->
+  Incorrectness (A1 ⊔ A2) p (C1 ⊔ C2).
+Proof. ikat. Qed.
+
+(** *** Identity (skp) *)
+Lemma rule_iskp A: Incorrectness A skp A.
+Proof.
+  rewrite Incorrectness_eq. intros s' HA. exists s'; [ exact HA | reflexivity ].
+Qed.
+
+(** *** Composition
+
+   This is the key rule that requires the [⊤·⊤ ≡ ⊤] axiom of TopKAT
+   ([top_nnm] in this development). *)
+Lemma rule_iseq A B C p q:
+  Incorrectness A p B ->
+  Incorrectness B q C ->
+  Incorrectness A (p;;q) C.
+Proof.
+  intros Hp Hq. simp.
+  transitivity ((top: hrel state state) ⋅ [B] ⋅ bstep q). exact Hq.
+  transitivity ((top: hrel state state) ⋅ (top ⋅ [A] ⋅ bstep p) ⋅ bstep q).
+  - now rewrite Hp.
+  - rewrite <-!dotA. rewrite (dotA (top: hrel state state) top).
+    rewrite top_nnm. reflexivity.
+Qed.
+
+(** *** Choice for [ite]: incorrectness can be discharged by either branch *)
+Lemma rule_iite_t A C t p q:
+  Incorrectness (A ⊓ t) p C ->
+  Incorrectness A (ite t p q) C.
+Proof.
+  rewrite !Incorrectness_eq. intros H s' HC.
+  destruct (H s' HC) as [s HAt Hp]. simpl in HAt.
+  apply Bool.andb_true_iff in HAt as [HA Ht].
+  exists s. exact HA.
+  simpl. left. exists s. split. reflexivity. simpl. exact Ht. exact Hp.
+Qed.
+
+Lemma rule_iite_f A C t p q:
+  Incorrectness (A ⊓ !t) q C ->
+  Incorrectness A (ite t p q) C.
+Proof.
+  rewrite !Incorrectness_eq. intros H s' HC.
+  destruct (H s' HC) as [s HAt Hp]. simpl in HAt.
+  apply Bool.andb_true_iff in HAt as [HA Ht].
+  exists s. exact HA.
+  simpl. right. exists s. split. reflexivity. simpl. exact Ht. exact Hp.
+Qed.
+
+(** *** While: zero iterations
+   If we enter the loop with the loop-test already false, [whl t p]
+   acts as the identity, so the postcondition can be the precondition
+   conjuncted with the negated test. *)
+Lemma rule_iwhl_zero A t p:
+  Incorrectness (A ⊓ !t) (whl t p) (A ⊓ !t).
+Proof.
+  rewrite Incorrectness_eq. intros s' HAnt.
+  exists s'. exact HAnt.
+  simpl. simpl in HAnt. apply Bool.andb_true_iff in HAnt as [_ Hnt].
+  exists s'. apply (str_refl ([t] ⋅ bstep p)). reflexivity.
+  split. reflexivity. exact Hnt.
+Qed.
+
+(** *** While: dependent invariant (Iter-Dependent rule)
+   Generalisation of the loop rule, indexed over the number of
+   iterations. Given an invariant family [I] such that each iteration
+   strengthens the invariant, after [n] iterations of the body we can
+   reach a state in [I n]; if additionally the loop test fails there,
+   we have exited the loop with postcondition [I n ⊓ !t]. *)
+
+(** Auxiliary fact: we can extend an iteration of length [n] by one
+    more step at the end. *)
+Lemma iter_extend (r: hrel state state) (n: nat) s0 sn s':
+  iter state r n s0 sn -> r sn s' -> iter state r (S n) s0 s'.
+Proof.
+  revert s0 sn s'. induction n as [|n IHn]; intros s0 sn s' Hiter Hr.
+  - simpl in Hiter. subst sn. simpl. exists s'. exact Hr. reflexivity.
+  - simpl in Hiter. destruct Hiter as [s1 Hr1 Hiter1].
+    simpl. exists s1. exact Hr1. apply (IHn _ _ _ Hiter1 Hr).
+Qed.
+
+Lemma rule_iwhl_dep (I: nat -> dset state) t p:
+  (forall n, Incorrectness (I n ⊓ t) p (I (S n))) ->
+  forall n, Incorrectness (I 0%nat) (whl t p) (I n ⊓ !t).
+Proof.
+  intros Hp n. rewrite Incorrectness_eq.
+  (* Helper: any state in [I n] is reachable from some state in [I 0]
+     in exactly [n] iterations of [t]·bstep p. *)
+  assert (Hloop: forall k s', I k s' = true ->
+            exists2 s0, I 0%nat s0 = true & iter state ([t]⋅bstep p) k s0 s').
+  { induction k as [|k IHk]; intros s' HI.
+    - exists s'. exact HI. simpl. reflexivity.
+    - specialize (Hp k). rewrite Incorrectness_eq in Hp.
+      destruct (Hp s' HI) as [sk HIkt Hpk]. simpl in HIkt.
+      apply Bool.andb_true_iff in HIkt as [HIk Ht].
+      destruct (IHk sk HIk) as [s0 HI0 Hiter].
+      exists s0. exact HI0.
+      apply (iter_extend _ _ _ sk).
+      + exact Hiter.
+      + exists sk. split. reflexivity. exact Ht. exact Hpk. }
+  intros s' HInt. simpl in HInt.
+  apply Bool.andb_true_iff in HInt as [HIn Hnt].
+  destruct (Hloop n s' HIn) as [s0 HI0 Hiter].
+  exists s0. exact HI0. simpl.
+  exists s'. exists n. exact Hiter. split. reflexivity. exact Hnt.
+Qed.
+
+(** *** Assignment
+
+   O'Hearn's assignment rule
+       [B] x := e [∃ y, B[y/x] ∧ x = e[y/x]]
+   uses a fresh syntactic variable [y] to capture the previous value
+   of [x]. Like its Hoare counterpart [rule_aff], this rule is
+   non-propositional: it goes beyond the equational theory of TopKAT.
+
+   Hoare and Incorrectness are however not symmetric here. For Hoare,
+   one can compute the strongest precondition by *backward*
+   substitution, which is a function ([subst]), so [rule_aff] is a
+   clean schema. For Incorrectness, one needs the strongest
+   *postcondition*, i.e. the image of the precondition through
+   [x := v], which is intrinsically existential.
+
+   In our semantic setting [dset state = state -> bool] there is no
+   way to express such an existential as a test in general. We
+   therefore state the rule as a soundness lemma whose hypothesis is
+   exactly the image side-condition: every state satisfying the
+   postcondition [C] must be exhibited as the result of running
+   [x := v] on some state in [B]. *)
+Lemma rule_iaff x v (B C: dset state):
+  (forall s', C s' = true ->
+              exists2 s, B s = true & s' = update x (v s) s) ->
+  Incorrectness B (x <- v) C.
+Proof.
+  rewrite Incorrectness_eq. intros H s' HC.
+  destruct (H s' HC) as [s HB Heq].
+  exists s. exact HB. simpl. unfold frel. now symmetry.
+Qed.
+
+End s.
+
+
