theories/KatInc_Imp.v
@@ -1,0 +1,129 @@
+(** * Connection: KatInc's KAT-based incorrectness logic ↔ Inc.v's semantic
+    IncTriple, in IMP's [com] / [store].
+
+    [prog'] mirrors KatInc's [prog] but with syntactic [aexp]/[bexp], so the
+    translation [to_com : prog' → com] (and [to_kat : prog' → prog]) is total.
+    We show that KatInc's relational semantics [bstep] coincides with IMP's
+    [cexec] on normal results, then lift [Incorrectness] to [IncTriple]. *)
+
+From Stdlib Require Import Program.Equality.
+From IncLogic Require Import Imp Sequences Hoare Inc KatInc.
+From RelationAlgebra Require Import rel.
+
+Local Open Scope string_scope.
+Local Open Scope Z_scope.
+Local Open Scope com_scope.
+
+(** ** A copy of KatInc's prog using syntactic expressions/tests. *)
+Inductive prog' : Type :=
+| skp'  : prog'
+| aff'  : ident -> aexp -> prog'
+| seq'  : prog' -> prog' -> prog'
+| ite'  : bexp -> prog' -> prog' -> prog'
+| whl'  : bexp -> prog' -> prog'.
+
+(** ** Translation to IMP's [com] (richer language). *)
+Fixpoint to_com (p: prog') : com :=
+  match p with
+  | skp'         => SKIP
+  | aff' x a     => ASSIGN x a
+  | seq' p q     => to_com p ;; to_com q
+  | ite' b p q   => CHOICE (ASSUME b ;; to_com p) (ASSUME (NOT b) ;; to_com q)
+  | whl' b p     => (((ASSUME b ;; to_com p) ★) ;; ASSUME (NOT b))
+  end.
+
+(** ** Translation to KatInc's [prog], specialised at [store]. *)
+Fixpoint to_kat (p: prog') : prog ident store :=
+  match p with
+  | skp'         => skp ident store
+  | aff' x a     => aff ident store x (aeval a)
+  | seq' p q     => seq ident store (to_kat p) (to_kat q)
+  | ite' b p q   => ite ident store (fun s => beval b s) (to_kat p) (to_kat q)
+  | whl' b p     => whl ident store (fun s => beval b s) (to_kat p)
+  end.
+
+(** ** KatInc's [bstep] at our chosen instantiation. *)
+Definition kat_bstep (p: prog') : hrel store store :=
+  bstep ident store Imp.update (to_kat p).
+
+(** ** From KatInc's inductive semantics to IMP's [cexec]. *)
+
+(** Helper: a [whl b body] derivation in [bstep'] produces a Kleene-star
+    chain of [(ASSUME b ;; body)] iterations ending in a [b]-false state. *)
+Lemma whl_to_star :
+  forall (b: bexp) (kbody: prog ident store) (cbody: com),
+    (forall s s',
+       bstep' ident store Imp.update kbody s s' ->
+       cexec s cbody (RNormal s')) ->
+    forall s s',
+    bstep' ident store Imp.update
+      (whl ident store (fun s => beval b s) kbody) s s' ->
+    star (step_iter (ASSUME b ;; cbody)) s s' /\ beval b s' = false.
+Proof.
+  intros b kbody cbody IHbody.
+  fix REC 3.
+  intros s s' HW.
+  inversion HW; subst.
+  - (* s_whl_ff *) split; [ apply star_refl | exact H3 ].
+  - (* s_whl_tt *)
+    inversion H4; subst.
+    destruct (REC _ _ H6) as [STAR Hbf].
+    split; [| exact Hbf ].
+    eapply star_step; [| exact STAR ].
+    unfold step_iter.
+    eapply cexec_seq;
+      [ apply cexec_assume; assumption | apply IHbody; assumption ].
+Qed.
+
+Lemma bstep'_to_cexec : forall p' s s',
+  bstep' ident store Imp.update (to_kat p') s s' ->
+  cexec s (to_com p') (RNormal s').
+Proof.
+  induction p'; intros s s' H; cbn in *.
+  - inversion H; subst; apply cexec_skip.
+  - inversion H; subst; apply cexec_assign.
+  - inversion H; subst.
+    eapply cexec_seq; [ apply IHp'1; eassumption | apply IHp'2; eassumption ].
+  - (* ite' *)
+    inversion H; subst.
+    + apply cexec_choice_right.
+      eapply cexec_seq.
+      * apply cexec_assume. cbn. now rewrite H5.
+      * apply IHp'2; assumption.
+    + apply cexec_choice_left.
+      eapply cexec_seq.
+      * apply cexec_assume; assumption.
+      * apply IHp'1; assumption.
+  - (* whl' *)
+    destruct (whl_to_star _ _ _ IHp' _ _ H) as [STAR Hbfalse].
+    apply cexec_cstar_iff_star in STAR.
+    eapply cexec_seq.
+    + exact STAR.
+    + apply cexec_assume. cbn. now rewrite Hbfalse.
+Qed.
+
+Lemma kat_bstep_to_cexec : forall p s s',
+  kat_bstep p s s' -> cexec s (to_com p) (RNormal s').
+Proof.
+  intros p s s' H.
+  unfold kat_bstep in H.
+  apply (bstep_eq ident store Imp.update) in H.
+  eapply bstep'_to_cexec; eauto.
+Qed.
+
+(** ** The main connection: Incorrectness ⇒ IncTriple.
+
+    We use [Incorrectness_eq] from [KatInc.v] to expose the semantic
+    formulation: every [C]-state is reachable from a [B]-state via [bstep]. *)
+Theorem Incorrectness_to_IncTriple :
+  forall (B C : store -> bool) (p : prog'),
+    (forall s', C s' = true ->
+                exists2 s, B s = true & kat_bstep p s s') ->
+    ⟦⟦ fun s => B s = true ⟧⟧ (to_com p) ⟦⟦ ok ↑ fun s => C s = true ⟧⟧.
+Proof.
+  intros B C p INC r HC.
+  destruct r as [s' | s']; [| exfalso; exact HC ].
+  destruct (INC s' HC) as [s HB Hp].
+  exists s. split; [ exact HB | ].
+  apply kat_bstep_to_cexec. exact Hp.
+Qed.
